theories/semantics.v
@@ -6,16 +6,27 @@ Require Import vec.
 Definition value := option nat.
 
 Definition stack := nat -> value.
-Definition heap := { n & vec n nat }.
+Definition heap := { n & vec n value }.
 
 Definition newptr (h : heap) : heap * nat :=
   match h with
-  | existT _ n l => (existT _ (S n) (append l 0) , n)
+  | existT _ n l => (existT _ (S n) (append l None) , n)
   end.
 
-Definition read (h : heap) (n : nat) : value :=
+Definition read (h : heap) (i : nat) : option value :=
   match h with
-  | existT _ n l => lookup l n
+  | existT _ _ l => lookup l i
+  end.
+
+Definition hasptr (h : heap) (i : nat) : Prop :=
+  match h with
+  | existT _ n _ => i < n
+  end.
+
+Definition write (h : heap) (i : nat) (v : value) : heap :=
+  match h with
+  | existT _ n l =>
+      existT _ n (update l i v)
   end.
 
 Definition state := ((stack * heap) + unit)%type.
@@ -38,37 +49,67 @@ Definition eval_expr (e : expr) (s : stack) : value :=
   | Null => None
   end.
 
+Definition isnat (s : stack) (e : expr) (n : nat) : Prop :=
+  match eval_expr e s with
+  | None => False
+  | Some n' => n = n'
+  end.
+
+Definition mapsto (h : heap) (i : nat) (v : value) : Prop :=
+  match read h i with
+  | None => False
+  | Some v' => v = v'
+  end.
+
+Definition is_true (v : value) : Prop :=
+  match v with
+  | Some n => n > 0
+  | None => False
+  end.
+
+Definition is_false (v : value) : Prop :=
+  match v with
+  | Some n => n = 0
+  | None => True
+  end.
+
 Inductive eval_cmd : cmd -> state -> state -> Prop :=
-| EvalAssume e s h n :
-  eval_expr e s = Some n ->
-  n > 0 ->
+| EvalAssume e s h v :
+  eval_expr e s = v ->
+  is_true v ->
   eval_cmd e <{s, h}> <{s, h}>
-| EvalNot e s h n :
-  eval_expr e s = Some n ->
-  n = 0 ->
+| EvalNot e s h v :
+  eval_expr e s = v ->
+  is_false v ->
   eval_cmd e <{s, h}> <{s, h}>
 | EvalAssign x e s s' h :
   s' = insert x (eval_expr e s) s ->
   eval_cmd (x <- e) <{s, h}> <{s', h}>
-| EvalAlloc x s s' h h' n :
-  (h' , n) = newptr h ->
-  s' = insert x (Some n) s ->
+| EvalAlloc x s s' h h' i :
+  (h' , i) = newptr h ->
+  s' = insert x (Some i) s ->
   eval_cmd (x <- alloc) <{s, h}> <{s', h'}>
-| EvalRead x e s s' h n n' :
-  eval_expr e s = Some n ->
-  read h n = Some n' ->
-  s' = insert x (Some n') s ->
+| EvalRead x e s s' h i v :
+  isnat s e i ->
+  mapsto h i v ->
+  s' = insert x v s ->
   eval_cmd (x <- [ e ]) <{s, h}> <{s', h}>
 | EvalReadNull x e s h :
   eval_expr e s = None ->
   eval_cmd (x <- [ e ]) <{s, h}> err
-| EvalReadInvalidPtr x e s h n :
-  (* todo: change heap to nat -> nat OR change heap to finite map *)
-  eval_expr e s = Some n ->
-  read h n = None ->
-  eval_cmd (x <- [ e ]) <{s, h}> err
-(* TODO: eval write, eval write error *)
+| EvalWrite e1 e2 s h h' i v :
+  isnat s e1 i ->
+  eval_expr e2 s = v ->
+  hasptr h i ->
+  h' = write h i v ->
+  eval_cmd ([ e1 ] <- e2) <{s, h}> <{s, h'}>
+| EvalWriteNull e1 e2 s h :
+  eval_expr e1 s = None ->
+  eval_cmd ([ e1 ] <- e2) <{s, h}> err
 .
+
+Hint Resolve EvalAssume EvalNot EvalAssign EvalAlloc EvalRead
+  EvalReadNull EvalWrite EvalWriteNull : core.
 
 Reserved Notation "x ⇓ y" (at level 80).
 
